to_node 와 to_node_list 가 bijection 이라는 것 부터 확실하게 해야 할 듯!

src/study/Nemonuri.Study.CSharpSyntaxRewriter2.Modifier2/Nemonuri.StratifiedNodes.Indexes.fst
@@ -6,23 +6,102 @@ module C = Nemonuri.StratifiedNodes.Children
 module Common = Nemonuri.StratifiedNodes.Common
 
 //--- theory members ---
-private let rec to_indexes_core #t (hd:N.node t) (tl:C.ancestor_list t) 
+private let rec get_indexes_core #t (hd:N.node t) (tl:C.ancestor_list t) 
   : Pure (list nat) 
     (requires (C.is_concatenatable_to_ancestor_list hd tl))
-    (ensures fun r -> true)
+    (ensures fun r -> 
+      (L.length r) = (L.length tl)
+    )
+    (decreases tl)
   =
   match tl with
   | [] -> []
-  | hd2::tl2 -> 
+  | hd2::tl2 -> (
+      assert (C.is_parent hd2 hd);
+      (C.get_child_index hd2 hd)::
+      (get_indexes_core hd2 tl2)
+  )
 
-let to_indexes #t (ancestors:C.ancestor_list t)
+let get_indexes #t (ancestors:C.ancestor_list t)
   : Pure (list nat) 
     (requires (Cons? ancestors)) 
-    (ensures fun r -> true)
+    (ensures fun r -> 
+      (L.length r) = ((L.length ancestors) - 1)
+    )
   =
   let hd::tl = ancestors in
-  match tl with
-  | [] -> []
-  | 
+  get_indexes_core hd tl
+
+(*
+private let rec are_indexes_of_core #t
+  (indexes:list nat)
+  (ancestors_hd:N.node t) (ancestors_tl:C.next_head_given_ancestor_list ancestors_hd)
+  : Pure bool 
+    (requires (L.length indexes) = (L.length ancestors_tl))
+    (ensures fun _ -> true)
+    (decreases indexes)
+  =
+  match ancestors_tl with
+  | [] -> true
+  | a_hd2::a_tl2 -> (
+      assert (C.is_parent a_hd2 ancestors_hd);
+      let i_hd::i_tl = indexes in
+      match ((C.get_child_index a_hd2 ancestors_hd) = i_hd) with
+      | false -> false
+      | true -> (are_indexes_of_core i_tl a_hd2 a_tl2)
+    )
+
+let are_indexes_of #t 
+  (indexes:list nat) (ancestors:C.ancestor_list t) 
+  : Pure bool
+    (requires (L.length indexes) = ((L.length ancestors) - 1))
+    (ensures fun _ -> true)
+    (decreases indexes)
+  =
+  let a_hd::a_tl = ancestors in
+  are_indexes_of_core indexes a_hd a_tl
+*)
+
+private let rec can_get_descendant_or_self_from_indexes_core #t
+  (hd:N.node t) (reversed_indexes:list nat)
+  : Tot bool (decreases reversed_indexes) =
+  if (not ((N.get_level hd) > (L.length reversed_indexes))) then
+    false
+  else if (L.isEmpty reversed_indexes) then
+    true
+  else
+    let children_length = (N.get_children_length hd) in
+    let child_index::next_reversed_indexes = reversed_indexes in
+    if (child_index < children_length) then (
+      let next_hd = (N.get_child_at hd child_index) in
+      can_get_descendant_or_self_from_indexes_core next_hd next_reversed_indexes
+    ) else false
+
+let can_get_descendant_or_self_from_indexes #t 
+  (hd:N.node t) (indexes:list nat)
+  : Tot bool =
+  can_get_descendant_or_self_from_indexes_core hd (L.rev indexes)
+
+private let rec get_descendant_or_self_from_indexes_core #t
+  (hd:N.node t) (reversed_indexes:list nat)
+  : Pure (N.node t)
+    (requires can_get_descendant_or_self_from_indexes_core hd reversed_indexes)
+    (ensures fun _ -> true)
+    (decreases reversed_indexes)
+  =
+  if (L.isEmpty reversed_indexes) then hd
+  else
+    let children_length = (N.get_children_length hd) in
+    let child_index::next_reversed_indexes = reversed_indexes in
+    let next_hd = (N.get_child_at hd child_index) in
+    get_descendant_or_self_from_indexes_core next_hd next_reversed_indexes
+
+let get_descendant_or_self_from_indexes #t
+  (hd:N.node t) (indexes:list nat)
+  : Pure (N.node t)
+    (requires can_get_descendant_or_self_from_indexes hd indexes)
+    (ensures fun _ -> true)
+  =
+  get_descendant_or_self_from_indexes_core hd (L.rev indexes)
 
 //---|
