src/study/Nemonuri.Study.CSharpSyntaxRewriter2.Modifier2/Nemonuri.StratifiedNodes.Nodes.fst
@@ -32,7 +32,18 @@ let get_value #t (node:node t) : Tot t = node.internal.value
 let get_children #t (node:node t) : Tot (node_list t) =
   to_node_list node.internal.children
 
-let get_children_length #t (node:node t) : Tot nat = I.get_length node.internal.children
+let get_children_length #t (node:node t) 
+  : Pure nat (requires True) (ensures fun r -> r = L.length (get_children node)) = 
+  assume (I.get_length node.internal.children = L.length (get_children node));
+  I.get_length node.internal.children
+
+let get_child_at #t (nd:node t) (index:nat)
+  : Pure (node t) 
+    (requires (index < (get_children_length nd)))
+    (ensures fun r -> r = (L.index (get_children nd) index))
+  =
+  // TODO: Internals 단계에서 구현하기
+  L.index (get_children nd) index
 
 let is_leaf #t (node:node t) : Tot bool = I.SNil? node.internal.children
 
