src/study/Nemonuri.Study.CSharpSyntaxRewriter2.Modifier2/Nemonuri.StratifiedNodes.Internals.fst
@@ -54,6 +54,9 @@ let get_level
 let get_max_level
   #t #max_level (nl:node_list_internal t max_level) : Tot nat =
   max_level
+
+//let get_element_at
+//  #t #max_level 
 //---|
 
 //--- proofs ---
